src/Variables/VariablesImpl.v
@@ -13,7 +13,7 @@ Module Vars <: VarsAPI.
 
   Axiom abstr : Abstraction State.
 
-  Axiom init_ok : init_invariant init recover abstr inited_any.
+  Axiom init_ok : init_abstraction init recover abstr inited_any.
   Axiom read_ok : forall v, prog_spec (read_spec v) (read v) recover abstr.
   Axiom write_ok : forall v val, prog_spec (write_spec v val) (write v val) recover abstr.
   Axiom recover_noop : rec_noop recover abstr no_crash.
